Add spec for TLUL

firmware/IncrementWait/CavaIncrementDevice.v
@@ -9,6 +9,7 @@ From Cava Require Import
      Expr
      Primitives
      Semantics
+     TLUL
      Types
      Util.BitArithmetic.
 
@@ -20,83 +21,414 @@ Section Var.
 
   Local Open Scope N.
 
-  (* Things that should probably be in cava *)
-  Section Cava.
-    Definition state_of {i s o} (c : Circuit s i o) := denote_type s.
-  End Cava.
+  Definition incr_state := BitVec 2.
+  Definition Idle       := Constant incr_state 0.
+  Definition Busy1      := Constant incr_state 1.
+  Definition Busy2      := Constant incr_state 2.
+  Definition Done       := Constant incr_state 3.
 
   Definition incr
-    : Circuit _
-              (* Input *)
-              [ Bit          (* is_read_req *)
-                ; Bit        (* is_write_req *)
-                ; BitVec 32  (* req_addr (only relevant if is_read_req or is_write_req) *)
-                ; BitVec 32 ](* req_value (only relevant if is_write_req *)
-              (* Output *)
-              (Bit             (* is_resp *)
-                 ** BitVec 32) (* resp (only relevant if is_resp *)
+    : Circuit _ [tl_h2d_t] tl_d2h_t
     := {{
-      fun is_read_req is_write_req req_addr req_value =>
-        (* bit #2 of the address determines if STATUS or VALUE register *)
-        let is_value_addr := (req_addr & (`K 1` << 2)) == `K 0` in
-        let is_value_write_req := is_value_addr && is_write_req in
-        let is_value_read_req := is_value_addr && is_read_req in
+      fun tl_h2d =>
+        (* Destruct and reconstruct tl_h2d with a_address that matches the
+           tlul_adapter_reg interface. *)
+        let '(a_valid
+              , a_opcode
+              , a_param
+              , a_size
+              , a_source
+              , a_address
+              , a_mask
+              , a_data
+              , a_user
+              ; d_ready) := tl_h2d in
+        (* Bit #2 of the address determines if STATUS or VALUE register. We zero
+           out all the rest. *)
+        let a_address := a_address & (`K 1` << 2) in
+        let tl_h2d := (a_valid
+                       , a_opcode
+                       , a_param
+                       , a_size
+                       , a_source
+                       , a_address
+                       , a_mask
+                       , a_data
+                       , a_user
+                       , d_ready) in
 
-        let/delay '(idle, busy, done; value) :=
-           if busy == `K 1` then
-             (`Zero`, `K 2`, `Zero`, value)
-           else if busy == `K 2` then
-                  (`Zero`, `K 0`, `One`, value + `K 1`)
-                else if done then
-                       (is_value_read_req, `K 0`, !is_value_read_req, value)
-                     else (* idle *)
-                       let busy' := if is_value_write_req then `K 1` else `K 0` in
-                       (!is_value_write_req, busy', `Zero`, req_value)
-           initially (false, (0, (false ,0))) : denote_type (Bit ** BitVec 2 ** Bit ** BitVec 32)
+        let/delay '(istate, value; tl_d2h) :=
+           let '(_, _, _, _, _, _, _, _, _; a_ready) := tl_d2h in
+
+           (* Compute the value of the status register *)
+           let status :=
+               if istate == `Done` then `K 4`
+               else if istate == `Busy1` || istate == `Busy2` then `K 2`
+                    else (* istate == `Idle` *) `K 1` in
+
+           let '(tl_d2h'; req) := `tlul_adapter_reg` tl_h2d (value :> status :> []) in
+
+           let '(is_write
+                 , _write_addr
+                 , write_data
+                 ; _write_mask) := req in
+
+           let is_value_read_req := a_valid
+                                    && a_ready
+                                    && a_opcode == `Get`
+                                    && a_address == `K 0` in
+
+           let istate' :=
+               if istate == `Busy1` then `Busy2`
+               else if istate == `Busy2` then `Done`
+                    else if istate == `Done` then
+                           if is_value_read_req then `Idle` else `Done`
+                         else (* istate == `Idle` *)
+                           if is_write then `Busy1` else `Idle` in
+
+           let value' :=
+               if istate == `Busy2` then value + `K 1`
+               else if istate == `Idle` then write_data
+                    else value in
+
+           (istate', value', tl_d2h')
+             initially (0,
+                        (0,
+                         (false, (0, (0, (0, (0, (0, (0, (0, (false, false)))))))))))
+           : denote_type (incr_state ** BitVec 32 ** tl_d2h_t)
         in
 
-        let status := if done then `K 1` else `K 0` in
-        let status := (status << 1) | (if busy == `K 0` then `K 0` else `K 1`) in
-        let status := (status << 1) | (if idle then `K 1` else `K 0`) in
-
-        let is_resp := is_read_req || is_write_req in
-        let resp := if is_value_addr then value else status in
-        (is_resp, resp)
+        tl_d2h
        }}.
 End Var.
 
+Section TLUL.
+  Record tl_h2d_t := mk_tl_h2d_t {
+                         a_valid : bool
+                         ; a_opcode : N
+                         ; a_param : N
+                         ; a_size : N
+                         ; a_source : N
+                         ; a_address : N
+                         ; a_mask : N
+                         ; a_data : N
+                         ; a_user : N
+                         ; d_ready : bool
+                       }.
+  Record tl_d2h_t := mk_tl_d2h_t {
+                         d_valid : bool
+                         ; d_opcode : N
+                         ; d_param : N
+                         ; d_size : N
+                         ; d_source : N
+                         ; d_sink : N
+                         ; d_data : N
+                         ; d_user : N
+                         ; d_error : bool
+                         ; a_ready : bool
+                       }.
+End TLUL.
+
 Example sample_trace :=
-  Eval compute in simulate incr
-                           [ (false,    (false, (111%N, (111%N, tt)))) (* no action *)
-                             ; (false,  (true,  (  0%N, ( 15%N, tt)))) (* write VALUE:=15 *)
-                             ; (true,   (false, (  4%N, (111%N, tt)))) (* read STATUS *)
-                             ; (true,   (false, (  4%N, (111%N, tt)))) (* read STATUS *)
-                             ; (true,   (false, (  0%N, (111%N, tt)))) (* read VALUE *)
-                           ].
+  Eval compute in
+    let nop :=
+        ((false,        (* a_valid   *)
+          (0,           (* a_opcode  *)
+           (0,          (* a_param   *)
+            (0,         (* a_size    *)
+             (0,        (* a_source  *)
+              (0,       (* a_address *)
+               (0,      (* a_mask    *)
+                (0,     (* a_data    *)
+                 (0,    (* a_user    *)
+                  (true (* d_ready   *)
+         )))))))))), tt)%N in
 
-Definition incr_device_step s (input : bool * bool * N * N) : (_ * (bool * N)) :=
-  let '(is_read_req, is_write_req, req_addr, req_value) := input in
-  step incr s (is_read_req,
-               (is_write_req,
-                (req_addr, (req_value, tt)))).
+    let read_reg (r : N) :=
+        ((true,         (* a_valid   *)
+          (4,           (* a_opcode  Get *)
+           (0,          (* a_param   *)
+            (0,         (* a_size    *)
+             (0,        (* a_source  *)
+              (r,       (* a_address *)
+               (0,      (* a_mask    *)
+                (0,     (* a_data    *)
+                 (0,    (* a_user    *)
+                  (true (* d_ready   *)
+         )))))))))), tt)%N in
 
-Require Import coqutil.Datatypes.List.
+    let write_val (v : N) :=
+        ((true,         (* a_valid   *)
+          (0,           (* a_opcode  PutFullData *)
+           (0,          (* a_param   *)
+            (0,         (* a_size    *)
+             (0,        (* a_source  *)
+              (0,       (* a_address value-reg *)
+               (0,      (* a_mask    *)
+                (v,     (* a_data    *)
+                 (0,    (* a_user    *)
+                  (true (* d_ready   *)
+         )))))))))), tt)%N in
+
+    simulate incr
+             [ nop
+               ; read_reg 4 (* status *)
+               ; nop
+               ; write_val 42
+               ; nop
+               ; nop
+               ; read_reg 4 (* status *)
+               ; nop
+               ; read_reg 0 (* value *)
+               ; nop
+               ; read_reg 4 (* status *)
+             ]%N.
+Print sample_trace.
+(* d_valid;  *)
+(* d_opcode; *)
+(* d_param;  *)
+(* d_size;   *)
+(* d_source; *)
+(* d_sink;   *)
+(* d_data;   *)
+(* d_user;   *)
+(* d_error;  *)
+(* a_ready;  *)
 
 Require Import Coq.ZArith.ZArith. Open Scope Z_scope.
+
 Require Import riscv.Utility.Utility.
+
+Require Import coqutil.Datatypes.List.
 Require Import coqutil.Map.Interface coqutil.Map.Properties.
 Require Import coqutil.Word.Interface coqutil.Word.Properties.
 Require Import coqutil.Tactics.Tactics.
 Require Import coqutil.Tactics.Simp.
+
 Require Import bedrock2.ZnWords.
+
 Require Import Bedrock2Experiments.RiscvMachineWithCavaDevice.InternalMMIOMachine.
 Require Import Bedrock2Experiments.IncrementWait.Constants.
 Require Import Bedrock2Experiments.IncrementWait.IncrementWaitSemantics.
 Require Import Bedrock2Experiments.StateMachineSemantics.
 Require Import Bedrock2Experiments.RiscvMachineWithCavaDevice.MMIOToCava.
 
+Require Import Cava.Expr.
+Require Import Cava.ExprProperties.
+Require Import Cava.Primitives.
+Require Import Cava.Semantics.
+Require Import Cava.Types.
 Require Import Cava.Util.Identity.
+Require Import Cava.Util.If.
+Require Import Cava.Util.List.
+Require Import Cava.Util.Nat.
 Require Import Cava.Util.Tactics.
+
+Section TLULProperties.
+  Local Open Scope bool_scope.
+  Local Open Scope N_scope.
+
+  Variant op :=
+  | Read
+  | Write (data : N).
+
+  (* State invariant *)
+  Definition tlul_adapter_reg_invariant
+             (state :  denote_type (BitVec 8 ** BitVec 2 ** BitVec 3 ** Bit ** Bit ** Bit ** Bit))
+             (* ghost *)
+    : Prop :=
+    let '(reqid, (reqsz, (rspop, (error, (outstanding, (we_o, re_o)))))) := state in
+    error = false.
+
+  (* Precondition *)
+  Definition tlul_adapter_reg_pre {reg_count}
+             (input : denote_type [TLUL.tl_h2d_t; Vec (BitVec 32) reg_count])
+             (* ghost *)
+             index op
+    : Prop :=
+    let '(incoming_tlp, (registers, tt)) := input in
+    let '(a_valid,
+          (a_opcode,
+           (_a_param,
+            (a_size,
+             (a_source,
+              (a_address,
+               (a_mask,
+                (a_data,
+                 (_a_user,
+                  d_ready))))))))) := incoming_tlp in
+    (* if a_valid then *)
+      List.length registers = reg_count /\
+      N.shiftr a_address 2 < N.of_nat reg_count /\
+      (* (a_opcode = 0 \/ a_opcode = 4) /\ *)
+      N.shiftl (N.of_nat index) 2 = a_address /\
+      (* index = N.to_nat (N.shiftr a_address 2) /\ *)
+      ((a_opcode = 0 /\ op = Write a_data) \/
+       (* a_opcode = 1 \/ a_opcode = 2 \/ a_opcode = 3 \/ *)
+       (a_opcode = 4 /\ op = Read)).
+    (* else True. *)
+
+  Definition tlul_adapter_reg_spec {reg_count}
+             (input : denote_type [TLUL.tl_h2d_t; Vec (BitVec 32) reg_count])
+             (state :  denote_type (BitVec 8 ** BitVec 2 ** BitVec 3 ** Bit ** Bit ** Bit ** Bit))
+             (* ghost *)
+             index op
+    : denote_type (TLUL.tl_d2h_t ** io_req) :=
+    let '(incoming_tlp, (registers, tt)) := input in
+    let '(reqid, (reqsz, (rspop, (error, (outstanding, (_we_o, _re_o)))))) := state in
+
+    let '(a_valid,
+          (_a_opcode,
+           (_a_param,
+            (a_size,
+             (a_source,
+              (a_address,
+               (a_mask,
+                (a_data,
+                 (_a_user,
+                  d_ready))))))))) := incoming_tlp in
+
+    if outstanding then
+      ((negb d_ready,
+        (rspop,
+         (0,
+          (reqsz,
+           (reqid,
+            (0,
+             (List.nth index registers 0,
+              (0,
+               (error,
+                d_ready))))))))),
+       (false, (a_address, (a_data, a_mask))))
+    else if a_valid then
+           ((true,
+             (match op with | Read => 1 | Write _ => 0 end (* if a_opcode =? 4 then 1 else 0 *),
+              (0,
+               (a_size,
+                (a_source,
+                 (0,
+                  (List.nth index registers 0,
+                   (0,
+                    (false,
+                     false))))))))),
+            match op with
+            | Write data => (true, (N.shiftl (N.of_nat index) 2, (data, a_mask)))
+            | _ => (false, (a_address, (a_data, a_mask)))
+            end)
+         else
+           ((false,
+             (rspop,
+              (0,
+               (reqsz,
+                (reqid,
+                 (0,
+                  (List.nth index registers 0,
+                   (0,
+                    (error,
+                     true))))))))),
+            (false, (a_address, (a_data, a_mask)))).
+
+  Lemma step_tlul_adapter_reg_invariant {reg_count}
+        (input : denote_type [TLUL.tl_h2d_t; Vec (BitVec 32) reg_count])
+        (state :  denote_type (BitVec 8 ** BitVec 2 ** BitVec 3 ** Bit ** Bit ** Bit ** Bit))
+        (* ghost *)
+        (index : nat) (op : op) :
+    tlul_adapter_reg_pre input index op ->
+    tlul_adapter_reg_invariant state ->
+    tlul_adapter_reg_invariant
+      (fst (Semantics.step TLUL.tlul_adapter_reg state input)).
+  Proof.
+    destruct input as (incoming_tlp, (registers, [])).
+    destruct incoming_tlp as (a_valid, (a_opcode, (a_param, (a_size, (a_source, (a_address, (a_mask, (a_data, (a_user, d_ready))))))))).
+    destruct state as (reqid, (reqsz, (rspop, (error, (outstanding, (we_o, re_o)))))).
+    cbv [tlul_adapter_reg_invariant tlul_adapter_reg_pre].
+    intros ? Hinv. logical_simplify. clear H. subst.
+    cbv [tlul_adapter_reg K]. stepsimpl.
+    repeat (destruct_pair_let; cbn [fst snd]).
+    autorewrite with tuple_if; cbn [fst snd].
+    cbn. destruct (a_valid && negb outstanding); reflexivity.
+  Qed.
+
+  Axiom denote_bv_max : forall (n : N) (m : denote_type (BitVec (N.to_nat n))),
+      m < 2 ^ n.
+
+  Lemma land_shiftr : forall (n v : N) (m : denote_type (BitVec (N.to_nat n))),
+      0 < n -> v <= n ->
+      N.land (N.shiftr m v) (2 ^ (n - v) - 1) = N.shiftr m v.
+  Proof.
+    intros. rewrite <- ? N.pred_sub. rewrite <- ? N.ones_equiv.
+    rewrite <- N.ones_div_pow2; auto. rewrite <- N.shiftr_div_pow2.
+    rewrite <- N.shiftr_land. rewrite N.land_ones_low. 1: reflexivity.
+    destruct m.
+    - (* 0 = m *) simpl. assumption.
+    - (* 0 < m *) apply N.log2_lt_pow2. 1: Lia.lia. apply denote_bv_max.
+  Qed.
+
+  Lemma shiftl_shiftr : forall n n' m,
+      N.shiftl n m = n' -> n = N.shiftr n' m.
+  Proof.
+    intros. apply f_equal with (f := fun x => N.shiftr x m) in H.
+    rewrite <- H. rewrite N.shiftr_shiftl_l; try Lia.lia. rewrite N.sub_diag.
+    rewrite N.shiftl_0_r. reflexivity.
+  Qed.
+
+  Lemma step_tlul_adapter_reg {reg_count}
+        (input : denote_type [TLUL.tl_h2d_t; Vec (BitVec 32) reg_count])
+        (state :  denote_type (BitVec 8 ** BitVec 2 ** BitVec 3 ** Bit ** Bit ** Bit ** Bit))
+        (* ghost *)
+        (index : nat) (op : op) :
+    tlul_adapter_reg_pre input index op ->
+    tlul_adapter_reg_invariant state ->
+    snd (step tlul_adapter_reg state input) = tlul_adapter_reg_spec input state index op.
+  Proof.
+    destruct input as (incoming_tlp, (registers, [])).
+    destruct incoming_tlp as (a_valid, (a_opcode, (a_param, (a_size, (a_source, (a_address, (a_mask, (a_data, (a_user, d_ready))))))))).
+    destruct state as (reqid, (reqsz, (rspop, (error, (outstanding, (we_o, re_o)))))).
+    destruct outstanding eqn:Eoutstanding.
+    - (* outstanding = true *)
+      cbv [tlul_adapter_reg_invariant tlul_adapter_reg_pre tlul_adapter_reg_spec].
+      intros. logical_simplify.
+      cbn. repeat (destruct_pair_let; cbn [fst snd]).
+      boolsimpl.
+      autorewrite with tuple_if; cbn [fst snd].
+      rewrite <- Bool.negb_if. rewrite <- Bool.andb_lazy_alt. boolsimpl.
+      repeat (rewrite pair_equal_spec).
+      ssplit; try reflexivity.
+      push_resize.
+      apply shiftl_shiftr in H2. apply f_equal with (f := N.to_nat) in H2.
+      rewrite Nnat.Nat2N.id in H2. subst index.
+      rewrite ? N.div2_spec.
+      rewrite N.shiftr_shiftr. cbn -[N.shiftr].
+      rewrite <- land_shiftr with (n := 32) (v := 2) at 2; try Lia.lia; []. reflexivity.
+    - (* outstanding = false *)
+      cbv [tlul_adapter_reg_invariant tlul_adapter_reg_pre tlul_adapter_reg_spec].
+      intros. logical_simplify.
+      cbn. repeat (destruct_pair_let; cbn [fst snd]).
+      boolsimpl.
+      autorewrite with tuple_if; cbn [fst snd].
+      destruct a_valid eqn:Ea_valid.
+      + (* a_valid = true *)
+        repeat (rewrite pair_equal_spec).
+        ssplit; try reflexivity; [| |].
+        * boolsimpl. clear H. destruct H3 as [H3 | H3]; destruct H3; subst; auto.
+        * push_resize.
+          apply shiftl_shiftr in H2. apply f_equal with (f := N.to_nat) in H2.
+          rewrite Nnat.Nat2N.id in H2. subst index.
+          rewrite ? N.div2_spec.
+          rewrite N.shiftr_shiftr. cbn -[N.shiftr].
+          rewrite <- land_shiftr with (n := 32) (v := 2) at 2; try Lia.lia; []. reflexivity.
+        * boolsimpl. clear H. destruct H3 as [H3 | H3]; destruct H3; subst; auto.
+      + (* a_valid = false *)
+        repeat (rewrite pair_equal_spec).
+        ssplit; try reflexivity; [].
+        push_resize.
+        apply shiftl_shiftr in H2. apply f_equal with (f := N.to_nat) in H2.
+        rewrite Nnat.Nat2N.id in H2. subst index.
+        rewrite ? N.div2_spec.
+        rewrite N.shiftr_shiftr. cbn -[N.shiftr].
+        rewrite <- land_shiftr with (n := 32) (v := 2) at 2; try Lia.lia; []. reflexivity.
+  Qed.
+End TLULProperties.
 
 Section WithParameters.
   Instance var : tvar := denote_type.
@@ -104,12 +436,55 @@ Section WithParameters.
   Context {word: Interface.word 32} {word_ok: word.ok word}
           {Mem: map.map word byte} {Registers: map.map Z word}.
 
-  Definition mk_counter_state idle busy done (val : N) : state_of incr :=
-    (idle, (busy, (done, val))).
+  Definition incr_device_step s '((is_read_req, is_write_req, req_addr, req_value) : (bool * bool * N * N))
+    : _ * (bool * N) :=
+    let input := ((is_read_req || is_write_req,     (* a_valid   *)
+                   (if is_read_req then 4 else 0, (* a_opcode  *)
+                    (0,                           (* a_param   *)
+                     (0,                          (* a_size    *)
+                      (0,                         (* a_source  *)
+                       (req_addr,                 (* a_address *)
+                        (0,                       (* a_mask    *)
+                         (req_value,              (* a_data    *)
+                          (0,                     (* a_user    *)
+                           true                   (* d_ready   *)
+                  ))))))))), tt)%N%bool in
+    let '(s', output) := Semantics.step incr s input in
+    let '(d_valid,
+          (_d_opcode,
+           (_d_param,
+            (_d_size,
+             (_d_source,
+              (_d_sink,
+               (d_data,
+                (_d_user,
+                 (_d_error,
+                  _a_ready))))))))) := output in
+    (s', (d_valid, d_data)).
+
+  Definition tl_d2h_of_tlul_state '((reqid, (reqsz, (rspop, (error, (outstanding, (_we_o, _re_o)))))) : (N * (N * (N * (bool * (bool * (bool * bool)))))))
+             (v : N) :=
+    (outstanding,
+     (rspop,
+      (0,
+       (reqsz,
+        (reqid,
+         (0,
+          (v,
+           (0,
+            (error,
+             (negb outstanding
+    ))))))))))%N.
+
+  Definition mk_counter_state (istate : N) (val : N) tl_d2h tlul_state
+    : denote_type (state_of incr) :=
+    ((istate, (val, tl_d2h)), tlul_state).
 
   Global Instance counter_device: device := {|
-    device.state := state_of incr;
-    device.is_ready_state s := exists val idle, s = mk_counter_state idle 0 false val;
+    device.state := denote_type (state_of incr);
+    device.is_ready_state s := exists val ival tl_d2h tlul_state,
+        tl_d2h = tl_d2h_of_tlul_state tlul_state ival
+        /\ s = mk_counter_state 0 val tl_d2h tlul_state;
     device.run1 := incr_device_step;
     device.addr_range_start := INCR_BASE_ADDR;
     device.addr_range_pastend := INCR_END_ADDR;
@@ -120,26 +495,27 @@ Section WithParameters.
   Global Instance circuit_spec : circuit_behavior :=
   {| ncycles_processing := 15%nat |}.
 
-  Ltac destruct_state s :=
-    destruct s as (?idle & ?busy & ?done & ?value).
-
-  Inductive counter_related: IncrementWaitSemantics.state -> state_of incr -> Prop :=
-  | IDLE_related: forall val idle,
-      (* after reset, all three bools are false, and idle will be set to true *)
-      counter_related IDLE (mk_counter_state idle 0 false val)
-  | BUSY1_related: forall val ncycles,
+  Inductive counter_related: IncrementWaitSemantics.state -> denote_type (state_of incr) -> Prop :=
+  | IDLE_related: forall val ival tl_d2h tlul_state,
+      tl_d2h = tl_d2h_of_tlul_state tlul_state ival ->
+      counter_related IDLE (mk_counter_state 0 val tl_d2h tlul_state)
+  | BUSY1_related: forall val ival tl_d2h tlul_state ncycles,
       (1 < ncycles)%nat ->
-      counter_related (BUSY val ncycles) (mk_counter_state false 1 false (word_to_N val))
-  | BUSY2_related: forall val ncycles,
+      tl_d2h = tl_d2h_of_tlul_state tlul_state ival ->
+      counter_related (BUSY val ncycles) (mk_counter_state 1 (word_to_N val) tl_d2h tlul_state)
+  | BUSY2_related: forall val ival tl_d2h tlul_state ncycles,
       (0 < ncycles)%nat ->
-      counter_related (BUSY val ncycles) (mk_counter_state false 2 false (word_to_N val))
+      tl_d2h = tl_d2h_of_tlul_state tlul_state ival ->
+      counter_related (BUSY val ncycles) (mk_counter_state 2 (word_to_N val) tl_d2h tlul_state)
   (* the hardware is already done, but the software hasn't polled it yet to find out,
      so we have to relate a software-BUSY to a hardware-done: *)
-  | BUSY_done_related: forall val ncycles,
+  | BUSY_done_related: forall val ival tl_d2h tlul_state ncycles,
+      tl_d2h = tl_d2h_of_tlul_state tlul_state ival ->
       counter_related (BUSY val ncycles)
-                      (mk_counter_state false 0 true (word_to_N (word.add (word.of_Z 1) val)))
-  | DONE_related: forall val,
-      counter_related (DONE val) (mk_counter_state false 0 true (word_to_N val)).
+                      (mk_counter_state 3 (word_to_N (word.add (word.of_Z 1) val)) tl_d2h tlul_state)
+  | DONE_related: forall val ival tl_d2h tlul_state,
+      tl_d2h = tl_d2h_of_tlul_state tlul_state ival ->
+      counter_related (DONE val) (mk_counter_state 3 (word_to_N val) tl_d2h tlul_state).
 
   (* This should be in bedrock2.ZnWords. It is use by ZnWords, which is used in
      the two following Lemmas. *)
@@ -155,6 +531,21 @@ Section WithParameters.
 
   Set Printing Depth 100000.
 
+  Ltac destruct_pair_let_hyp :=
+    match goal with
+    | H: context [ match ?p with
+                   | pair _ _ => _
+                   end ] |- _ =>
+      destruct p as [?p0 ?p1] eqn:?H0
+    end.
+
+  Ltac destruct_pair_equal_hyp :=
+    match goal with
+    | H: context [ (?l0, ?l1) = (?r0, ?r1) ] |- _ =>
+      eapply pair_equal_spec in H; destruct H as [?H0 ?H1]
+    end.
+
+  (* Set Printing All. *)
   Global Instance cava_counter_satisfies_state_machine:
     device_implements_state_machine counter_device increment_wait_state_machine.
   Proof.
@@ -163,29 +554,56 @@ Section WithParameters.
     - (* mmioAddrs_match: *)
       reflexivity.
     - (* initial_state_is_ready_state: *)
-      simpl in *. subst. inversion H0. eauto.
+      simpl in *. subst. inversion H0. do 4 eexists. subst. eauto.
     - (* initial_states_are_related: *)
-      simpl in *. destruct H0 as (val & idle & H0). subst. eapply IDLE_related.
+      simpl in *. destruct H0 as (val & ival & tl_d2h & tlul_state & H0 & H1). subst.
+      eauto using IDLE_related.
     - (* initial_state_exists: *)
-      simpl in *. destruct H as (val & idle & H). subst. eauto using IDLE_related.
+      simpl in *. destruct H as (val & ival & tl_d2h & tlul_state & H0 & H1). subst.
+      eauto using IDLE_related.
     - (* nonMMIO_device_step_preserves_state_machine_state: *)
-      simpl in sL1, sL2. destruct_state sL1. destruct_state sL2.
-      cbn in H0. simp.
+      simpl in sL1, sL2.
+      cbn in H0.
+      (* simp. *)
+      repeat destruct_pair_let_hyp. (* <-- very slow *)
+      repeat (destruct_pair_equal_hyp; subst; cbn).
       inversion H; subst; simp;
         (* try rewrite N.land_0_r; *)
         try rewrite Bool.andb_false_r;
+        unfold tl_d2h_of_tlul_state in *;
         cbn.
       + (* IDLE_related: *)
-        apply IDLE_related.
+        eapply IDLE_related.
+        rewrite Bool.andb_true_r. rewrite <- Bool.negb_if.
+        rewrite <- Bool.andb_lazy_alt. rewrite Bool.andb_negb_l.
+        simpl.
+        repeat (apply pair_equal_spec; split; try reflexivity).
       + (* BUSY1_related: *)
-        apply BUSY2_related. Lia.lia.
+        eapply BUSY2_related.
+        * Lia.lia.
+        * rewrite Bool.andb_true_r. rewrite <- Bool.negb_if.
+          rewrite <- Bool.andb_lazy_alt. rewrite Bool.andb_negb_l.
+          simpl.
+          repeat (apply pair_equal_spec; split; try reflexivity).
       + (* BUSY2_related: *)
         rewrite incrN_word_to_bv.
-        apply BUSY_done_related.
+        eapply BUSY_done_related.
+        rewrite Bool.andb_true_r. rewrite <- Bool.negb_if.
+        rewrite <- Bool.andb_lazy_alt. rewrite Bool.andb_negb_l.
+        simpl.
+        repeat (apply pair_equal_spec; split; try reflexivity).
       + (* BUSY_done_related: *)
-        apply BUSY_done_related.
+        eapply BUSY_done_related.
+        rewrite Bool.andb_true_r. rewrite <- Bool.negb_if.
+        rewrite <- Bool.andb_lazy_alt. rewrite Bool.andb_negb_l.
+        simpl.
+        repeat (apply pair_equal_spec; split; try reflexivity).
       + (* DONE_related: *)
-        apply DONE_related.
+        eapply DONE_related.
+        rewrite Bool.andb_true_r. rewrite <- Bool.negb_if.
+        rewrite <- Bool.andb_lazy_alt. rewrite Bool.andb_negb_l.
+        simpl.
+        repeat (apply pair_equal_spec; split; try reflexivity).
     - (* state_machine_read_to_device_read: *)
       (* simpler because device.maxRespDelay=1 *)
       unfold device.maxRespDelay, device.runUntilResp, device.state, device.run1, counter_device.
@@ -194,11 +612,15 @@ Section WithParameters.
       unfold read_step in *.
       destruct r.
       + (* r=VALUE *)
-        simp. cbn. rewrite Z_word_N; try Lia.lia; []. cbn.
-        unfold word_to_N.
-        (* rewrite word.unsigned_of_Z_nowrap by (cbv; intuition discriminate). *)
-        simpl. do 3 eexists. ssplit; try reflexivity.
-        eapply IDLE_related.
+        simp. cbn.
+        destruct tlul_state as [reqid [reqsz [rspop [error [outstanding [we_o re_o]]]]]].
+        (* destruct tl_d2h as [d_valid [d_opcode [d_param [d_size [d_source [d_sink [d_data [d_user [d_error a_ready]]]]]]]]]. *)
+        cbn.
+        destruct outstanding; [|];
+          rewrite Z_word_N; try Lia.lia;
+            (* rewrite word.unsigned_of_Z_nowrap by (cbv; intuition discriminate). *)
+            do 3 eexists; ssplit; try reflexivity;
+              eapply IDLE_related; reflexivity.
       + (* r=STATUS *)
         destruct sH.
         * (* sH=IDLE *)
@@ -206,24 +628,39 @@ Section WithParameters.
           cbn. repeat (rewrite Z_word_N; try Lia.lia; []; cbn).
           unfold status_value, STATUS_IDLE, word_to_N.
           (* rewrite word.unsigned_of_Z_nowrap by (cbv; intuition discriminate). *)
-          do 3 eexists. ssplit; try reflexivity. 2: eapply IDLE_related.
-          rewrite word.unsigned_slu. 2: rewrite word.unsigned_of_Z. 2: reflexivity.
-          rewrite !word.unsigned_of_Z. unfold word.wrap. cbn.
-          destruct idle; reflexivity.
+          do 3 eexists. ssplit; try reflexivity.
+          -- rewrite word.unsigned_slu; try ZnWords; [].
+             rewrite !word.unsigned_of_Z. unfold word.wrap. cbn.
+             destruct tlul_state as [reqid [reqsz [rspop [error [outstanding [we_o re_o]]]]]].
+             destruct outstanding; reflexivity.
+          -- simpl. eapply IDLE_related. reflexivity.
         * (* sH=BUSY *)
-          simp. destruct Hp1 as [H | H].
+          destruct Hp1 as [H | H].
           -- (* transition to DONE *)
-             destruct H; subst.
+             destruct H. subst.
              simpl (state_machine.reg_addr _).
              unfold STATUS_ADDR, INCR_BASE_ADDR, word_to_N, status_value, STATUS_DONE.
              rewrite !word.unsigned_of_Z. unfold word.wrap. simpl.
-             inversion H0; subst.
+             inversion H0; subst; [| |].
              ++ (* BUSY1_related *)
-                destruct max_cycles_until_done. 1: inversion H3. clear H3.
-                exists (word.of_Z 2). (* <- bit #1 (busy) is set, all others are 0 *)
-                do 2 eexists.
-                rewrite !word.unsigned_of_Z. unfold word.wrap. cbn.
-                ssplit; try reflexivity.
+               destruct max_cycles_until_done; [|].
+               ** exfalso. eapply NPeano.Nat.nlt_0_r. apply H2.
+               **
+                  (* clear H0. *)
+                  exists (word.of_Z 2). (* <- bit #1 (busy) is set, all others are 0 *)
+                  do 2 eexists.
+                  destruct tlul_state as [reqid [reqsz [rspop [error [outstanding [we_o re_o]]]]]].
+                  cbn.
+                  rewrite !word.unsigned_of_Z. unfold word.wrap. cbn.
+                  ssplit; try reflexivity; [| |].
+                  { destruct outstanding; [|].
+                    { cbn. reflexivity. }
+                    { cbn. reflexivity. }
+                    admit. }
+                  { admit. }
+                  { right. exists max_cycles_until_done. ssplit; try reflexivity; []. ZnWords. }
+
+                 inversion H0; subst.
                 ** eapply BUSY2_related.
                    instantiate ( 1 := max_cycles_until_done ).
                    inversion H0; subst.
